
% Discussion with classmates: I discussed with Kapilan for all the homeworks. 

\subsection*{Problem 1.}

Let $X$ follows the exponential distribution with the rate parameter $\lambda$, then its (uncentered) MGF is
\begin{align*}
  E{\exp \del{tX}}
  % E{\exp \del{tX}} = \frac{ \lambda }{ - t} \; \forall t < \lambda
\end{align*}


We have

% \begin{align*}
  
%   \stackrel{r_2}{\le}\,
% \end{align*}

% In order to prove $g(x) \deq f(Ax + b)$ convex, we prove $g(x)$ satisfies $\forall x, y \in \RR^n$, $\forall \alpha \in [0, 1]$, $g(\alpha x + (1-\alpha)y) \le \alpha g(x) + (1-\alpha)g(y)$

% $\forall x, y \in \RR^n$, $\forall \alpha \in [0, 1]$, we have
% \begin{align*}
%   &g(\alpha x + (1-\alpha)y) \\
%   =\,& f(A(\alpha x + (1-\alpha)y) + b) && \mcmt{by definition of g(x)} \\
%   =\,& f(\alpha Ax + (1-\alpha)Ay + b) \\
%   =\,& f(\alpha(Ax + b) + (1-\alpha)(Ay + b)) \\
%   \le\,& \alpha f(Ax + b) + (1-\alpha)f(Ay + b) && \mcmt{apply convexity of $f$ with $Ax + b \in R^m$, $Ay + b \in R^m$, $\alpha \in [0, 1]$}\\
%   =\,& \alpha g(x) + (1-\alpha)g(y) && \mcmt{by definition of g(x)}
% \end{align*}

